Allow frozen pointer annotations to be refined.
The refinement relation on addresses allows union references to be refined:

  (β2 → β1) → RUnion i s β1 ⊆ RUnion i s β2

The result is that frozen values are below their unfrozen variant, which made
it possible to prove that constant propagation (see constant_propagation.v) can
be performed on the level of the memory model.

addresses_refine.v
@@ -4,28 +4,32 @@ Require Export addresses refinements.
 Require Import pointer_casts.
 Local Open Scope ctype_scope.
 
-Inductive ref_refine `{Env Ti} (r' : ref Ti) (sz : nat) :
-     ref Ti → nat → ref Ti → nat → Prop :=
-  | ref_refine_nil i :
-     ref_refine r' sz [] i (ref_base r') (i + sz * ref_offset r')
-  | ref_refine_ne_nil rs r i :
-     ref_refine r' sz (rs :: r) i (rs :: r ++ r') i.
+Inductive ref_refine `{Env Ti} (sz : nat) :
+     bool → ref Ti → ref Ti → nat → ref Ti → nat → Prop :=
+  | ref_refine_perm r i :
+     ref_refine sz false [] r i r i
+  | ref_refine_nil r1 i1 r2 i2 :
+     ref_base r1 ⊆* r2 → i2 = i1 + sz * ref_offset r1 →
+     ref_refine sz true r1 [] i1 r2 i2
+  | ref_refine_ne_nil r1' r1 r2 i :
+     r1 ++ r1' ⊆* r2 → r1 ≠ [] →
+     ref_refine sz true r1' r1 i r2 i.
 Inductive addr_refine' `{Env Ti} (Γ : env Ti) (α : bool) (f : meminj Ti)
       (Γm1 Γm2 : memenv Ti) : addr Ti → addr Ti → type Ti → Prop :=
-  | Addr_refine' o o' r r' r'' i i'' τ τ' σ σc :
+  | Addr_refine' o1 o2 r1 r' r2 i1 i2 τ1 τ2 σ σc :
      Γm1 ⊑{Γ,α,f} Γm2 →
-     f !! o = Some (o',r') →
-     Γm1 ⊢ o : τ →
-     ✓{Γ} τ' →
-     int_typed (size_of Γ τ') sptrT →
-     Γ ⊢ r' : τ' ↣ τ → Γ ⊢ r : τ ↣ σ →
-     ref_offset r = 0 →
-     i ≤ size_of Γ σ * ref_size r →
-     i `mod` size_of Γ σc = 0 →
+     f !! o1 = Some (o2,r') →
+     Γm1 ⊢ o1 : τ1 →
+     ✓{Γ} τ2 →
+     int_typed (size_of Γ τ2) sptrT →
+     Γ ⊢ r' : τ2 ↣ τ1 → Γ ⊢ r1 : τ1 ↣ σ →
+     ref_offset r1 = 0 →
+     i1 ≤ size_of Γ σ * ref_size r1 →
+     i1 `mod` size_of Γ σc = 0 →
      σ >*> σc →
-     ref_refine (freeze true <$> r') (size_of Γ σ) r i r'' i'' →
+     ref_refine (size_of Γ σ) α r' r1 i1 r2 i2 →
      addr_refine' Γ α f Γm1 Γm2
-       (Addr o r i τ σ σc) (Addr o' r'' i'' τ' σ σc) σc.
+       (Addr o1 r1 i1 τ1 σ σc) (Addr o2 r2 i2 τ2 σ σc) σc.
 Instance addr_refine `{Env Ti} :
   RefineT Ti (env Ti) (type Ti) (addr Ti) := addr_refine'.
 
@@ -36,14 +40,8 @@ Implicit Types Γm : memenv Ti.
 Implicit Types τ σ : type Ti.
 Implicit Types r : ref Ti.
 Implicit Types a : addr Ti.
+Implicit Types α : bool.
 
-Lemma ref_refine_nil_alt r' sz r'' i i' :
-  i' = i + sz * ref_offset r' → r'' = ref_base r' →
-  ref_refine r' sz [] i r'' i'.
-Proof. intros -> ->. by constructor. Qed.
-Lemma ref_refine_ne_nil_alt r' sz rs r r'' i :
-  r'' = rs :: r ++ r' → ref_refine r' sz (rs :: r) i r'' i.
-Proof. intros ->. by constructor. Qed.
 Lemma addr_refine_typed_l Γ α f Γm1 Γm2 a1 a2 σ :
   ✓ Γ → a1 ⊑{Γ,α,f@Γm1↦Γm2} a2 : σ → (Γ,Γm1) ⊢ a1 : σ.
 Proof.
@@ -58,26 +56,27 @@ Qed.
 Lemma addr_refine_typed_r Γ α f Γm1 Γm2 a1 a2 σ :
   ✓ Γ → a1 ⊑{Γ,α,f@Γm1↦Γm2} a2 : σ → (Γ,Γm2) ⊢ a2 : σ.
 Proof.
-  destruct 2 as [o o' r r' r'' i i'' τ τ' σ σc HΓm ?????????? Hr''].
-  assert (ref_offset (freeze true <$> r') < ref_size (freeze true <$> r')).
-  { intros. eapply ref_typed_size, ref_typed_freeze; eauto. }
+  destruct 2 as [o1 o2 r1 r' r2 i1 i2 τ1 τ2 σ σc HΓm ?????????? Hr].
+  assert (ref_offset r' < ref_size r') by eauto using ref_typed_size.
   constructor; auto.
-  * by destruct (memenv_refine_typed_l HΓm o o' r' τ) 
+  * by destruct (memenv_refine_typed_l HΓm o1 o2 r' τ1) 
       as (?&?&?); simplify_type_equality'.
-  * destruct Hr''; simplify_type_equality'.
-    + apply ref_set_offset_typed, ref_typed_freeze; auto with lia.
-    + rewrite app_comm_cons, ref_typed_app.
-      exists τ. by rewrite ref_typed_freeze.
-  * destruct Hr''; simplify_equality'; auto.
-    by rewrite ref_offset_set_offset by lia.
-  * destruct Hr''; simplify_equality'; auto. rewrite ref_size_set_offset.
-    transitivity (size_of Γ σ * S (ref_offset (freeze true <$> r'))); [lia|].
-    apply Nat.mul_le_mono_l; lia.
-  * destruct Hr''; simplify_equality'; auto.
+  * destruct Hr as [|r1 i1 r2 i2|r1' r1 r2 i]; simplify_type_equality'; auto.
+    + eapply ref_typed_le; [|eauto]. apply ref_set_offset_typed; auto with lia.
+    + eapply ref_typed_le; rewrite ?ref_typed_app; eauto.
+  * destruct Hr as [|r1 i1 r2 i2|r1' r1 r2 i]; simplify_equality'; auto.
+    + by erewrite <-ref_offset_le, ref_offset_set_offset by eauto with lia.
+    + erewrite <-ref_offset_le by eauto. by destruct r1.
+  * destruct Hr as [|r1 i1 r2 i2|r1' r1 r2 i]; simplify_equality'; auto.
+    + erewrite <-ref_size_le, ref_size_set_offset by eauto.
+      transitivity (size_of Γ σ * S (ref_offset r1)); [lia|].
+      apply Nat.mul_le_mono_l; lia.
+    + erewrite <-ref_size_le by eauto. by destruct r1.
+  * destruct Hr as [|r1 i1 r2 i2|r1' r1 r2 i]; simplify_equality'; auto.
     destruct (castable_divide Γ σ σc) as [z ->]; auto.
-    by rewrite <-Nat.mul_assoc, (Nat.mul_comm (size_of _ _)), Nat.mul_assoc,
-      Nat.mod_add by eauto using size_of_ne_0,
-      castable_type_valid, ref_typed_type_valid.
+    by rewrite <-Nat.mul_assoc,
+      (Nat.mul_comm (size_of _ _)), Nat.mul_assoc, Nat.mod_add
+      by eauto using size_of_ne_0, castable_type_valid, ref_typed_type_valid.
 Qed.
 Lemma addr_refine_type_of_l Γ α f Γm1 Γm2 a1 a2 σ :
   a1 ⊑{Γ,α,f@Γm1↦Γm2} a2 : σ → type_of a1 = σ.
@@ -86,117 +85,137 @@ Lemma addr_refine_type_of_r Γ α f Γm1 Γm2 a1 a2 σ :
   a1 ⊑{Γ,α,f@Γm1↦Γm2} a2 : σ → type_of a2 = σ.
 Proof. by destruct 1. Qed.
 Lemma addr_refine_frozen Γ α f Γm1 Γm2 a1 a2 σ :
-  a1 ⊑{Γ,α,f@Γm1↦Γm2} a2 : σ → frozen a1 ↔ frozen a2.
+  a1 ⊑{Γ,α,f@Γm1↦Γm2} a2 : σ → frozen a2 → frozen a1.
 Proof.
-  unfold frozen.
-  destruct 1 as [o o' r' r r'' i i'' τ τ' σ σc ??????????? []]; csimpl.
-  * by rewrite ref_set_offset_freeze, ref_freeze_freeze.
-  * rewrite fmap_app, ref_freeze_freeze.
-    by split; intro; simplify_list_equality; repeat f_equal.
+  unfold frozen. destruct 1 as [o1 o2 r1 r' r2 i1 i2 τ1 τ2 σ σc ??????????? Hr];
+    destruct Hr as [|r1 i1 r2 i2|]; intros; decompose_Forall_hyps;
+    f_equal; eauto using ref_frozen_le, ref_freeze_freeze.
+Qed.
+Lemma ref_refine_id sz α r i : ref_refine sz α [] r i r i.
+Proof.
+  destruct α; [|constructor].
+  destruct (decide (r = [])) as [->|];
+    constructor; csimpl; rewrite ?(right_id_L [] (++)); auto with lia.
 Qed.
 Lemma addr_refine_id Γ α Γm a σ : (Γ,Γm) ⊢ a : σ → a ⊑{Γ,α@Γm} a : σ.
 Proof.
   destruct 1 as [o r i τ σ σc].
-  eexists []; csimpl; auto using memenv_refine_id; [by apply ref_typed_nil|].
-  destruct r as [|rs r]; [apply ref_refine_nil_alt; csimpl; auto with lia|].
-  apply ref_refine_ne_nil_alt. by rewrite (right_id_L [] (++)).
+  eexists []; csimpl; auto using memenv_refine_id, ref_refine_id.
+  by apply ref_typed_nil.
 Qed.
 Lemma addr_refine_compose Γ α1 α2 f1 f2 Γm1 Γm2 Γm3 a1 a2 a3 σ σ' :
   ✓ Γ → a1 ⊑{Γ,α1,f1@Γm1↦Γm2} a2 : σ → a2 ⊑{Γ,α2,f2@Γm2↦Γm3} a3 : σ' →
   a1 ⊑{Γ,α1||α2,f2 ◎ f1@Γm1↦Γm3} a3 : σ.
 Proof.
-  destruct 2 as [o o2 r r2 r3 i i3 τ τ2 σ σc ??????????? Hr3];
-    inversion 1 as [? o4 ? r4 r5 ? i5 ? τ3 ????????????? Hr5]; subst.
-  exists (r2 ++ r4); eauto using memenv_refine_compose.
+  destruct 2 as [o1 o2 r1 r1' r2 i1 i2 τ1 τ2 σ σc ??????????? Hr3];
+    inversion 1 as [? o3 ? r2' r3 ? i3 ? τ3 ????????????? Hr5]; subst.
+  exists (r1' ++ r2'); eauto using memenv_refine_compose.
   { by rewrite lookup_meminj_compose; simplify_option_equality. }
   { rewrite ref_typed_app; eauto. }
-  destruct Hr3 as [?|rs r i]; inversion Hr5; subst.
-  * destruct r2; simplify_equality'. apply ref_refine_nil_alt; auto with lia.
-  * destruct r2; simplify_equality'.
-    by apply ref_refine_nil_alt; rewrite ?fmap_cons, ?fmap_app.
-  * apply ref_refine_ne_nil_alt. by rewrite fmap_app, (associative_L (++)).
+  destruct Hr3 as [r1 i|r1 i1 r2 i2|r1' r1 r2 i]; inversion Hr5;
+    simplify_type_equality'; rewrite ?(right_id_L [] (++)); try by constructor.
+  * destruct r1; decompose_Forall_hyps. constructor; auto with lia.
+  * destruct r1; decompose_Forall_hyps.
+    constructor; simpl; auto. constructor; [etransitivity; eauto|].
+    apply Forall2_app; [etransitivity; eauto|eauto].
+  * destruct r1; decompose_Forall_hyps.
+  * constructor; auto. transitivity (r2 ++ r2'); auto.
+    by rewrite (associative_L (++)); apply Forall2_app.
 Qed.
 Lemma addr_refine_inverse Γ f Γm1 Γm2 a1 a2 σ :
   a1 ⊑{Γ,false,f@Γm1↦Γm2} a2 : σ →
   a2 ⊑{Γ,false,meminj_inverse f@Γm2↦Γm1} a1 : σ.
 Proof.
-  destruct 1 as [o o' r r' r'' i i'' τ τ' σ σc ??????????? Hr].
-  destruct (memenv_refine_perm_l Γ f Γm1 Γm2 o τ)
+  destruct 1 as [o1 o2 r1 r' r2 i1 i2 τ1 τ2 σ σc ??????????? Hr].
+  inversion Hr; destruct (memenv_refine_perm_l Γ f Γm1 Γm2 o1 τ1)
     as (?&?&?); auto; simplify_type_equality'.
-  inversion Hr; simplify_equality'.
-  * refine_constructor; eauto using lookup_meminj_inverse_2,
-      memenv_refine_inverse, ref_typed_nil_2; simpl;
-      rewrite Nat.mul_0_r, Nat.add_0_r; auto.
-    apply ref_refine_nil_alt; simpl; auto with lia.
-  * rewrite (right_id_L [] (++)).
-    refine_constructor; eauto using lookup_meminj_inverse_2,
-      memenv_refine_inverse, ref_typed_nil_2.
-    apply ref_refine_ne_nil_alt; simpl. by rewrite (right_id_L [] (++)).
+  refine_constructor; eauto using lookup_meminj_inverse_2,
+    memenv_refine_inverse, ref_typed_nil_2.
 Qed.
 Lemma addr_refine_weaken Γ Γ' α α' f f' Γm1 Γm2 Γm1' Γm2' a1 a2 σ :
-  ✓ Γ → a1 ⊑{Γ,α,f@Γm1↦Γm2} a2 : σ → Γ ⊆ Γ' → Γm1' ⊑{Γ',α',f'} Γm2' →
+  ✓ Γ → a1 ⊑{Γ,α,f@Γm1↦Γm2} a2 : σ → Γ ⊆ Γ' → (α → α') → Γm1' ⊑{Γ',α',f'} Γm2' →
   Γm1 ⇒ₘ Γm1' → meminj_extend f f' Γm1 Γm2 → a1 ⊑{Γ',α',f'@Γm1'↦Γm2'} a2 : σ.
 Proof.
-  destruct 2 as [o o2 r r2 r3 i i3 τ τ2 σ σc]; intros ?? [??] [??];
-    econstructor; eauto using type_valid_weaken, ref_typed_weaken.
+  destruct 2 as [o1 o2 r1 r' r2 i1 i2 τ1 τ2 σ σc ??????????? Hr];
+    intros ??? [??] [??];
+    refine_constructor; eauto using type_valid_weaken, ref_typed_weaken.
   * eauto using option_eq_1_alt.
   * by erewrite <-size_of_weaken by eauto.
   * by erewrite <-size_of_weaken by eauto using ref_typed_type_valid.
   * by erewrite <-size_of_weaken
       by eauto using ref_typed_type_valid, castable_type_valid.
-  * by erewrite <-size_of_weaken by eauto using ref_typed_type_valid.
+  * erewrite <-size_of_weaken by eauto using ref_typed_type_valid.
+    destruct Hr, α'; csimpl in *; try tauto || constructor (done).
+    apply ref_refine_id.
 Qed.
 (* only holds for renamings because of end-of-array pointers *)
 Lemma addr_refine_unique_l Γ f Γm1 Γm2 a1 a2 a3 σ2 σ3 :
   a1 ⊑{Γ,false,f@Γm1↦Γm2} a3 : σ2 → a2 ⊑{Γ,false,f@Γm1↦Γm2} a3 : σ3 → a1 = a2.
 Proof.
   destruct 1 as [o1 o2 r r2 r3 i i3 τ τ2 σ σc ??? _ _ _ _ _ _ _ _ Hr];
-    inversion 1 as [o1' ? r' r2' ? i' ? τ' ??? _ ?? _ _ _ _ _ _ _ _ Hr'];
-    simplify_equality'.
-  destruct (memenv_refine_perm_l Γ f Γm1 Γm2 o1 τ) as (?&?&_),
-    (memenv_refine_perm_l Γ f Γm1 Γm2 o1' τ') as (?&?&_); auto;
-    simplify_equality.
-  destruct (meminj_injective_alt f o1 o1' o2 [] [])
-    as [?|[_ ?]]; eauto using memenv_refine_injective; simplify_type_equality;
-    [|by destruct (ref_disjoint_nil_inv_l (@nil (ref_seg Ti)))].
-  inversion Hr; inversion Hr'; simplify_list_equality; f_equal; lia.
+    inversion 1 as [o1' o2' r' r2' ? i' ? τ' ??? _ ?? _ _ _ _ _ _ _ _ Hr'];
+    inversion Hr; inversion Hr'; simplify_equality.
+  destruct (meminj_injective_alt f o1 o1' o2 [] []) as [?|[_ ?]];
+    eauto using memenv_refine_injective; simplify_type_equality; auto.
+  by destruct (ref_disjoint_nil_inv_l (@nil (ref_seg Ti))).
 Qed.
-Lemma addr_refine_unique_r Γ α α' f Γm1 Γm2 a1 a2 a3 σ2 σ3 :
-  a1 ⊑{Γ,α,f@Γm1↦Γm2} a2 : σ2 → a1 ⊑{Γ,α',f@Γm1↦Γm2} a3 : σ3 → a2 = a3.
+Lemma addr_refine_unique_r Γ α f Γm1 Γm2 a1 a2 a3 σ2 σ3 :
+  a1 ⊑{Γ,α,f@Γm1↦Γm2} a2 : σ2 → a1 ⊑{Γ,α,f@Γm1↦Γm2} a3 : σ3 →
+  frozen a2 → frozen a3 → a2 = a3.
 Proof.
-  destruct 1 as [?????????????????????? []];
-    inversion 1 as [?????????????????????? Hr2]; inversion Hr2;
-    simplify_type_equality'; naive_solver.
+  unfold frozen; destruct 1 as [?????????????????????? Hr1];
+    inversion 1 as [?????????????????????? Hr2]; destruct Hr1; inversion Hr2;
+    intros; simplify_type_equality'; f_equal; eauto using ref_le_unique_alt.
+Qed.
+Lemma addr_freeze_refine_l Γ Γm a σ :
+  (Γ,Γm) ⊢ a : σ → freeze true a ⊑{Γ,true@Γm} a : σ.
+Proof.
+  destruct 1. eexists []; csimpl; auto using memenv_refine_id.
+  * by apply ref_typed_nil.
+  * eauto using ref_typed_ge, ref_freeze_le_l.
+  * by rewrite ref_offset_freeze.
+  * by rewrite ref_size_freeze.
+  * destruct (decide (r = [])) as [->|]; [constructor; simpl; auto with lia|].
+    constructor. rewrite (right_id_L [] (++)); auto using ref_freeze_le_l.
+    by destruct r.
 Qed.
 Lemma addr_freeze_refine Γ α f Γm1 Γm2 a1 a2 σ :
   a1 ⊑{Γ,α,f@Γm1↦Γm2} a2 : σ →
   freeze true a1 ⊑{Γ,α,f@Γm1↦Γm2} freeze true a2 : σ.
 Proof.
-  intros Ha. destruct Ha as [o o' r r' r'' i i'' τ τ' σ σc ??????????? Hr''];
-    csimpl; econstructor; eauto;
-    rewrite ?ref_typed_freeze, ?ref_offset_freeze, ?ref_size_freeze; auto.
-  destruct Hr'' as [|r'' i'']; csimpl.
-  * eapply ref_refine_nil_alt; eauto.
-    by rewrite <-ref_set_offset_freeze, ref_freeze_freeze.
-  * eapply ref_refine_ne_nil_alt; eauto.
-    by rewrite fmap_app, ref_freeze_freeze.
+  destruct 1 as [o1 o2 r1 r' r2 i1 i2 τ1 τ2 σ σc HΓm ?????????? Hr];
+    csimpl; refine_constructor; eauto.
+  { by apply ref_typed_freeze. }
+  { by rewrite ref_offset_freeze. }
+  { by rewrite ref_size_freeze. }
+  destruct Hr as [|r1 i1 r2 i2|r1' r1 r2 i]; constructor; auto.
+  * erewrite <-(memenv_refine_frozen _ _ _ _ _ HΓm _ _ r1) by eauto.
+    by erewrite ref_set_offset_freeze, ref_freeze_le by eauto.
+  * erewrite <-(memenv_refine_frozen _ _ _ _ _ HΓm _ _ r1'), <-fmap_app by eauto.
+    by erewrite ref_freeze_le by eauto.
+  * by destruct r1.
 Qed.
 Lemma addr_ref_refine Γ α f Γm1 Γm2 a1 a2 σ :
   a1 ⊑{Γ,α,f@Γm1↦Γm2} a2 : σ → addr_strict Γ a1 →
-  ∃ r, f !! addr_index a1 = Some (addr_index a2, r)
-    ∧ addr_ref Γ a2 = addr_ref Γ a1 ++ freeze true <$> r.
+  ∃ r, f !! addr_index a1 = Some (addr_index a2, r) ∧
+    addr_ref Γ a1 ++ r ⊆* addr_ref Γ a2.
 Proof.
-  intros [?? r r' r'' i i'' τ τ' σ' ???????????? Hr''] ?; simplify_equality'.
-  exists r'; split; auto. destruct Hr''; simplify_equality'; auto.
-  rewrite Nat.mul_comm, Nat.div_add, Nat.div_small, Nat.add_0_l by lia.
-  by rewrite ref_set_offset_set_offset, ref_set_offset_offset.
+  destruct 1 as [o1 o2 r1 r' r2 i1 i2 τ1 τ2 σ' ???????????? Hr];
+    intros; simplify_equality'; exists r'; split; auto.
+  destruct Hr as [|r1 i1 r2 i2|r1' r1 r2 i]; simplify_type_equality'; auto.
+  * by rewrite (right_id_L [] (++)).
+  * rewrite Nat.mul_comm, Nat.div_add, Nat.div_small, Nat.add_0_l by lia.
+    rewrite <-(ref_set_offset_offset r1) at 1.
+    rewrite <-(ref_set_offset_set_offset r1 _ 0); auto using ref_set_offset_le.
+  * destruct r1; decompose_Forall_hyps.
+    constructor; auto using Forall2_app, ref_seg_set_offset_le.
 Qed.
 Lemma addr_ref_byte_refine Γ α f Γm1 Γm2 a1 a2 σ :
   a1 ⊑{Γ,α,f@Γm1↦Γm2} a2 : σ → addr_strict Γ a1 →
   addr_ref_byte Γ a1 = addr_ref_byte Γ a2.
 Proof.
-  intros [?? r r' r'' i i'' τ τ' σ' ???????????? Hr''] ?;
-    simplify_equality'; destruct Hr''; simplify_equality'; auto.
+  destruct 1 as [o1 o2 r1 r' r2 i1 i2 τ1 τ2 σ' ???????????? Hr];
+    intros; destruct Hr; simplify_equality'; auto.
   by rewrite Nat.mul_comm, Nat.mod_add by lia.
 Qed.
 Lemma addr_is_obj_refine Γ α f Γm1 Γm2 a1 a2 σ :
@@ -213,16 +232,17 @@ Proof.
   intros [?|[[Hidx ?]|(Hidx&Ha&?&?&?)]].
   * edestruct (meminj_injective_ne f (addr_index a1) (addr_index a2))
       as [|[??]]; eauto; [by left|].
-    right; left; split; [done|]. rewrite Hr1, Hr2.
-    by apply ref_disjoint_app, ref_disjoint_freeze_l, ref_disjoint_freeze_r.
-  * rewrite Hidx in Hf1; simplify_option_equality. right; left; split; auto.
-    rewrite Hr1, Hr2. by apply ref_disjoint_here_app_1.
+    right; left; eauto using ref_disjoint_le, ref_disjoint_app.
+  * rewrite Hidx in Hf1; simplify_option_equality.
+    right; left; eauto using ref_disjoint_le, ref_disjoint_here_app_1.
   * rewrite Hidx in Hf1; simplify_option_equality. do 2 right; split; [done|].
-    by erewrite Hr1, Hr2, !fmap_app, Ha,
-      <-!(addr_ref_byte_refine _ _ _ _ _ a1 a2),
+    erewrite <-!(addr_ref_byte_refine _ _ _ _ _ a1 a2),
       <-!(addr_ref_byte_refine _ _ _ _ _ a3 a4),
       <-!(addr_is_obj_refine _ _ _ _ _ a1 a2),
-      <-!(addr_is_obj_refine _ _ _ _ _ a3 a4) by eauto.
+      <-!(addr_is_obj_refine _ _ _ _ _ a3 a4) by eauto; split_ands; auto.
+    transitivity (freeze true <$> addr_ref Γ a1 ++ r1);
+      auto using ref_freeze_le, eq_sym.
+    rewrite fmap_app, Ha, <-fmap_app; auto using ref_freeze_le.
 Qed.
 Lemma addr_disjoint_refine_inv Γ α α' f Γm1 Γm2 a1 a2 a3 a4 σ1 σ3 :
   ✓ Γ → addr_strict Γ a1 → addr_strict Γ a3 →
@@ -235,14 +255,15 @@ Proof.
   destruct (decide (addr_index a1 = addr_index a3)) as [Hidx|]; [|by left].
   intros [?|[[Hidx' ?]|(Hidx'&Ha&?&?&?)]]; [congruence| |].
   * right; left; split; [done|]. rewrite Hidx in Hf1; simplify_equality.
-    apply ref_disjoint_here_app_2 with (freeze true <$> r1); congruence.
+    eauto using ref_disjoint_here_app_2, ref_disjoint_ge.
   * right; right; split; [done|]. rewrite Hidx in Hf1; simplify_equality.
     erewrite !(addr_ref_byte_refine _ _ _ _ _ a1 a2),
       !(addr_ref_byte_refine _ _ _ _ _ a3 a4),
       !(addr_is_obj_refine _ _ _ _ _ a1 a2),
       !(addr_is_obj_refine _ _ _ _ _ a3 a4) by eauto; split_ands; auto.
-    apply (injective (++ freeze true <$> freeze true <$> r1)).
-    rewrite <-!fmap_app. congruence.
+    apply (injective (++ freeze true <$> r1)); rewrite <-!fmap_app.
+    erewrite ref_freeze_le by eauto. rewrite Ha.
+    eauto using ref_freeze_le, eq_sym.
 Qed.
 Lemma addr_byte_refine_help Γ α f Γm1 Γm2 a1 a2 σ :
   a1 ⊑{Γ,α,f@Γm1↦Γm2} a2 : σ →
@@ -250,12 +271,15 @@ Lemma addr_byte_refine_help Γ α f Γm1 Γm2 a1 a2 σ :
     ≤ size_of Γ (addr_type_base a2) * ref_size (addr_ref_base a2)
   ∧ addr_byte a2 = i + addr_byte a1.
 Proof.
-  destruct 1 as [o o' r r' r'' i i'' τ τ' σ' σc ??????????? Hr''].
-  destruct Hr'' as [|r'' i'']; simplify_type_equality'; [|by exists 0].
-  rewrite ref_size_set_offset.
-  exists (size_of Γ σ' * ref_offset (freeze true <$> r')). split; [|lia].
-  rewrite <-Nat.mul_add_distr_l, Nat.add_comm. eapply Nat.mul_le_mono_l,
-    Nat.le_succ_l, ref_typed_size, ref_typed_freeze; eauto.
+  destruct 1 as [o1 o2 r1 r' r2 i1 i2 τ1 τ2 σ σc ??????????? Hr].
+  destruct Hr as [|r1 i1 r2 i2 Hr|r1' r1 r2 i]; simplify_type_equality'.
+  * by exists 0.
+  * exists (size_of Γ σ * ref_offset r1); split; [|lia].
+    erewrite <-(ref_size_le _ r2), ref_size_set_offset by eauto.
+    rewrite <-Nat.mul_add_distr_l, Nat.add_comm; apply Nat.mul_le_mono_l.
+    eapply Nat.le_succ_l, ref_typed_size; eauto.
+  * exists 0; split; auto. erewrite <-(ref_size_le _ r2) by eauto.
+    by destruct r1.
 Qed.
 Lemma addr_strict_refine Γ α f Γm1 Γm2 a1 a2 σ :
   a1 ⊑{Γ,α,f@Γm1↦Γm2} a2 : σ → addr_strict Γ a1 → addr_strict Γ a2.
@@ -272,11 +296,10 @@ Lemma addr_top_refine Γ α f Γm1 Γm2 o1 o2 τ :
   ✓{Γ} τ → int_typed (size_of Γ τ) sptrT →
   addr_top o1 τ ⊑{Γ,α,f@Γm1↦Γm2} addr_top o2 τ : τ.
 Proof.
-  econstructor; eauto using Nat.mod_0_l, size_of_ne_0.
+  econstructor; eauto using Nat.mod_0_l, size_of_ne_0, ref_refine_id.
   * by constructor.
   * by constructor.
   * simpl; lia.
-  * apply ref_refine_nil_alt; simpl; auto with lia.
 Qed.
 Lemma addr_top_array_refine Γ α f Γm1 Γm2 o1 o2 τ (n : Z) :
   ✓ Γ → Γm1 ⊑{Γ,α,f} Γm2 → Γm1 ⊢ o1 : τ.[Z.to_nat n] → f !! o1 = Some (o2,[]) →
@@ -290,6 +313,6 @@ Proof.
   * repeat typed_constructor; lia.
   * lia.
   * eauto using Nat.mod_0_l, size_of_ne_0.
-  * constructor.
+  * apply ref_refine_id.
 Qed.
 End addresses.
