pointers_refine.v
@@ -17,6 +17,7 @@ Section pointers.
 Context `{EnvSpec Ti}.
 Implicit Types Γ : env Ti.
 Implicit Types Γm : memenv Ti.
+Implicit Types α : bool.
 Implicit Types τ : type Ti.
 Implicit Types a : addr Ti.
 Implicit Types p : ptr Ti.
@@ -34,10 +35,10 @@ Lemma ptr_refine_type_of_r Γ α f Γm1 Γm2 p1 p2 σ :
   p1 ⊑{Γ,α,f@Γm1↦Γm2} p2 : σ → type_of p2 = σ.
 Proof. destruct 1; simpl; eauto using addr_refine_type_of_r. Qed.
 Lemma ptr_refine_frozen Γ α f Γm1 Γm2 p1 p2 σ :
-  p1 ⊑{Γ,α,f@Γm1↦Γm2} p2 : σ → frozen p1 ↔ frozen p2.
+  p1 ⊑{Γ,α,f@Γm1↦Γm2} p2 : σ → frozen p2 → frozen p1.
 Proof.
   unfold frozen. destruct 1; simpl; auto.
-  rewrite !(injective_iff Ptr). eapply (addr_refine_frozen Γ α f); eauto.
+  rewrite !(injective_iff Ptr). eapply addr_refine_frozen; eauto.
 Qed.
 Lemma ptr_refine_id Γ α Γm p σ : (Γ,Γm) ⊢ p : σ → p ⊑{Γ,α@Γm} p : σ.
 Proof. destruct 1; constructor; eauto using addr_refine_id. Qed.
@@ -52,7 +53,7 @@ Lemma ptr_refine_inverse Γ f Γm1 Γm2 p1 p2 σ :
   p2 ⊑{Γ,false,meminj_inverse f@Γm2↦Γm1} p1 : σ.
 Proof. destruct 1; constructor; eauto using addr_refine_inverse. Qed.
 Lemma ptr_refine_weaken Γ Γ' α α' f f' Γm1 Γm2 Γm1' Γm2' p1 p2 σ :
-  ✓ Γ → p1 ⊑{Γ,α,f@Γm1↦Γm2} p2 : σ → Γ ⊆ Γ' →
+  ✓ Γ → p1 ⊑{Γ,α,f@Γm1↦Γm2} p2 : σ → Γ ⊆ Γ' → (α → α') →
   Γm1' ⊑{Γ',α',f'} Γm2' → Γm1 ⇒ₘ Γm1' →
   meminj_extend f f' Γm1 Γm2 → p1 ⊑{Γ',α',f'@Γm1'↦Γm2'} p2 : σ.
 Proof.
@@ -65,10 +66,15 @@ Proof.
   destruct 1; inversion_clear 1; f_equal; eauto using addr_refine_unique_l.
 Qed.
 Lemma ptr_refine_unique_r Γ α f Γm1 Γm2 p1 p2 p3 σ2 σ3 :
-  p1 ⊑{Γ,α,f@Γm1↦Γm2} p2 : σ2 → p1 ⊑{Γ,α,f@Γm1↦Γm2} p3 : σ3 → p2 = p3.
+  p1 ⊑{Γ,α,f@Γm1↦Γm2} p2 : σ2 → p1 ⊑{Γ,α,f@Γm1↦Γm2} p3 : σ3 →
+  frozen p2 → frozen p3 → p2 = p3.
 Proof.
-  destruct 1; inversion_clear 1; f_equal; eauto using addr_refine_unique_r.
+  unfold frozen. destruct 1; inversion_clear 1; intros; simplify_equality';
+    f_equal; eauto using addr_refine_unique_r.
 Qed.
+Lemma ptr_freeze_refine_l Γ Γm p σ :
+  (Γ,Γm) ⊢ p : σ → freeze true p ⊑{Γ,true@Γm} p : σ.
+Proof. destruct 1; refine_constructor; eauto using addr_freeze_refine_l. Qed.
 Lemma ptr_freeze_refine Γ α f Γm1 Γm2 p1 p2 σ :
   p1 ⊑{Γ,α,f@Γm1↦Γm2} p2 : σ →
   freeze true p1 ⊑{Γ,α,f@Γm1↦Γm2} freeze true p2 : σ.
